Compiler/Erase.v
@@ -2,6 +2,7 @@ Require Stlc.SpecSyntax.
 Require Utlc.SpecSyntax.
 Require Import Stlc.SpecTyping.
 Require Import Stlc.LemmasTyping.
+Require Import Stlc.SpecEvaluation.
 Require Import Stlc.LemmasEvaluation.
 Require Import Utlc.SpecScoping.
 Require Import Utlc.LemmasScoping.
@@ -307,10 +308,10 @@ Section CompatibilityLemmas.
         (refine (S.eval_ctx₀ S.phole _ I); refine (S.eval_beta vvs₂)).
     assert (es1 : S.evaln (S.app (S.abs (repEmul τ₁) tsb) vs₂) (tsb [beta1 vs₂]) 1) by 
         (eauto using S.evaln; omega).
-    assert (eu : forall Cu, U.ECtx Cu → U.eval (U.pctx_app (U.app (U.abs tub) vu₂) Cu) (U.pctx_app (tub [beta1 vu₂]) Cu)) by
-        (intros Cu eCu; refine (U.eval_ctx₀ Cu _ eCu); refine (U.eval_beta vvu₂)).
-    assert (eu1 : forall Cu, U.ECtx Cu → U.evaln (U.pctx_app (U.app (U.abs tub) vu₂) Cu) (U.pctx_app (tub [beta1 vu₂]) Cu) 1) by 
-        (eauto using U.evaln; omega).
+    assert (eu : U.ctxeval (U.app (U.abs tub) vu₂) (tub [beta1 vu₂])) by
+        (refine (U.mkCtxEval phole _ _ I _); refine (U.eval_beta vvu₂)).
+    assert (eu1 : U.ctxevaln (U.app (U.abs tub) vu₂) (tub [beta1 vu₂]) 1) by 
+        (unfold U.ctxevaln; eauto with eval).
     destruct w; try apply termrel_zero.
     refine (termrel_antired w es1 eu1 _ _ _); unfold lev in *; simpl; try omega.
 
@@ -447,9 +448,10 @@ Section CompatibilityLemmas.
     assert (S.eval (S.proj₂ (S.pair vs₁ vs₂)) vs₂) by 
         (apply (S.eval_ctx₀ S.phole); try refine (S.eval_proj₂ _ _); simpl; intuition).
     assert (esn : S.evaln (S.proj₂ (S.pair vs₁ vs₂)) vs₂ 1) by eauto using S.evaln.
-    assert (forall Cu, U.ECtx Cu → U.eval (U.pctx_app (U.proj₂ (U.pair vu₁ vu₂)) Cu) (U.pctx_app vu₂ Cu)) by 
-        (intros Cu eCu; apply (U.eval_ctx₀ Cu); try refine (U.eval_proj₂ _); simpl; intuition).
-    assert (eun : forall Cu, U.ECtx Cu → U.evaln (U.pctx_app (U.proj₂ (U.pair vu₁ vu₂)) Cu) (U.pctx_app vu₂ Cu) 1) by eauto using U.evaln.
+    assert (U.ctxeval (U.proj₂ (U.pair vu₁ vu₂)) vu₂) by 
+        (apply (U.mkCtxEval phole); try refine (U.eval_proj₂ _); simpl; intuition).
+    assert (eun : U.ctxevaln (U.proj₂ (U.pair vu₁ vu₂)) vu₂ 1)
+           by (unfold U.ctxevaln; eauto with eval).
     destruct w'; try apply termrel_zero.
     refine (termrel_antired w' esn eun _ _ _); crush.
 
@@ -483,9 +485,9 @@ Section CompatibilityLemmas.
     assert (S.eval (S.proj₁ (S.pair vs₁ vs₂)) vs₁) by 
         (apply (S.eval_ctx₀ S.phole); try refine (S.eval_proj₁ _ _); simpl; intuition).
     assert (esn : S.evaln (S.proj₁ (S.pair vs₁ vs₂)) vs₁ 1) by eauto using S.evaln.
-    assert (forall Cu, U.ECtx Cu → U.eval (U.pctx_app (U.proj₁ (U.pair vu₁ vu₂)) Cu) (U.pctx_app vu₁ Cu)) by 
-        (intros Cu eCu; apply (U.eval_ctx₀ Cu); try refine (U.eval_proj₁ _); simpl; intuition).
-    assert (eun : forall Cu, U.ECtx Cu → U.evaln (U.pctx_app (U.proj₁ (U.pair vu₁ vu₂)) Cu) (U.pctx_app vu₁ Cu) 1) by eauto using U.evaln.
+    assert (U.ctxeval (U.proj₁ (U.pair vu₁ vu₂)) vu₁) by 
+        (apply (U.mkCtxEval phole); try refine (U.eval_proj₁ _); simpl; intuition).
+    assert (eun : U.ctxevaln (U.proj₁ (U.pair vu₁ vu₂)) vu₁ 1) by (unfold U.ctxevaln; eauto with eval).
     destruct w'; try apply termrel_zero.
     refine (termrel_antired w' esn eun _ _ _); crush.
 
@@ -521,16 +523,16 @@ Section CompatibilityLemmas.
     - assert (S.eval (S.ite S.true ts₂ ts₃) ts₂) by 
           (apply (S.eval_ctx₀ S.phole); try refine (S.eval_ite_true _ _); simpl; intuition).
       assert (esn : S.evaln (S.ite S.true ts₂ ts₃) ts₂ 1) by eauto using S.evaln.
-      assert (forall Cu, U.ECtx Cu → U.eval (U.pctx_app (U.ite U.true tu₂ tu₃) Cu) (U.pctx_app tu₂ Cu)) by 
-          (intros Cu eCu; apply (U.eval_ctx₀ Cu); try refine (U.eval_ite_true _ _); simpl; intuition).
-      assert (eun : forall Cu, U.ECtx Cu → U.evaln (U.pctx_app (U.ite U.true tu₂ tu₃) Cu) (U.pctx_app tu₂ Cu) 1) by eauto using U.evaln.
+      assert (U.ctxeval (U.ite U.true tu₂ tu₃) tu₂) by 
+          (apply (U.mkCtxEval phole); try refine (U.eval_ite_true _ _); simpl; intuition).
+      assert (eun : U.ctxevaln (U.ite U.true tu₂ tu₃) tu₂ 1) by (unfold U.ctxevaln; eauto with eval).
       refine (termrel_antired w' esn eun _ _ _); crush.
     - assert (S.eval (S.ite S.false ts₂ ts₃) ts₃) by 
           (apply (S.eval_ctx₀ S.phole); try refine (S.eval_ite_false _ _); simpl; intuition).
       assert (esn : S.evaln (S.ite S.false ts₂ ts₃) ts₃ 1) by eauto using S.evaln.
-      assert (forall Cu, U.ECtx Cu → U.eval (U.pctx_app (U.ite U.false tu₂ tu₃) Cu) (U.pctx_app tu₃ Cu)) by 
-          (intros Cu eCu; apply (U.eval_ctx₀ Cu); try refine (U.eval_ite_false _ _); simpl; intuition).
-      assert (eun : forall Cu, U.ECtx Cu → U.evaln (U.pctx_app (U.ite U.false tu₂ tu₃) Cu) (U.pctx_app tu₃ Cu) 1) by eauto using U.evaln.
+      assert (U.ctxeval (U.ite U.false tu₂ tu₃) tu₃) by 
+          (apply (U.mkCtxEval phole); try refine (U.eval_ite_false _ _); simpl; intuition).
+      assert (eun : U.ctxevaln (U.ite U.false tu₂ tu₃) tu₃ 1) by (unfold U.ctxevaln; eauto with eval).
       refine (termrel_antired w' esn eun _ _ _); crush.
   Qed. 
 
@@ -566,17 +568,17 @@ Section CompatibilityLemmas.
     - assert (S.eval (S.caseof (S.inl vs') ts₂ ts₃) (ts₂ [beta1 vs'])) by
           (apply (S.eval_ctx₀ S.phole); try refine (S.eval_case_inl _); simpl; intuition).
       assert (esn : S.evaln (S.caseof (S.inl vs') ts₂ ts₃) (ts₂ [beta1 vs']) 1) by eauto using S.evaln.
-      assert (forall Cu, U.ECtx Cu → U.eval (U.pctx_app (U.caseof (U.inl vu') tu₂ tu₃) Cu) (U.pctx_app (tu₂ [beta1 vu']) Cu)) by 
-          (intros Cu eCu; apply (U.eval_ctx₀ Cu); try refine (U.eval_case_inl _ _); simpl; intuition).
-      assert (eun : forall Cu, U.ECtx Cu → U.evaln (U.pctx_app (U.caseof (U.inl vu') tu₂ tu₃) Cu) (U.pctx_app (tu₂ [beta1 vu']) Cu) 1) by eauto using U.evaln.
+      assert (U.ctxeval (U.caseof (U.inl vu') tu₂ tu₃) (tu₂ [beta1 vu'])) by 
+          (apply (U.mkCtxEval phole); try refine (U.eval_case_inl _ _); simpl; intuition).
+      assert (eun : U.ctxevaln (U.caseof (U.inl vu') tu₂ tu₃) (tu₂ [beta1 vu']) 1) by (unfold U.ctxevaln; eauto with eval).
       destruct w'; try apply termrel_zero.
       refine (termrel_antired w' esn eun _ _ _); crush.
     - assert (S.eval (S.caseof (S.inr vs') ts₂ ts₃) (ts₃ [beta1 vs'])) by
           (apply (S.eval_ctx₀ S.phole); try refine (S.eval_case_inr _); simpl; intuition).
       assert (esn : S.evaln (S.caseof (S.inr vs') ts₂ ts₃) (ts₃ [beta1 vs']) 1) by eauto using S.evaln.
-      assert (forall Cu, U.ECtx Cu → U.eval (U.pctx_app (U.caseof (U.inr vu') tu₂ tu₃) Cu) (U.pctx_app (tu₃ [beta1 vu']) Cu)) by 
-          (intros Cu eCu; apply (U.eval_ctx₀ Cu); try refine (U.eval_case_inr _ _); simpl; intuition).
-      assert (eun : forall Cu, U.ECtx Cu → U.evaln (U.pctx_app (U.caseof (U.inr vu') tu₂ tu₃) Cu) (U.pctx_app (tu₃ [beta1 vu']) Cu) 1) by eauto using U.evaln.
+      assert (U.ctxeval (U.caseof (U.inr vu') tu₂ tu₃) (tu₃ [beta1 vu'])) by 
+          (apply (U.mkCtxEval phole); try refine (U.eval_case_inr _ _); simpl; intuition).
+      assert (eun : U.ctxevaln (U.caseof (U.inr vu') tu₂ tu₃) (tu₃ [beta1 vu']) 1) by (unfold U.ctxevaln; eauto with eval).
       destruct w'; try apply termrel_zero.
       refine (termrel_antired w' esn eun _ _ _); crush.
   Qed. 
@@ -618,8 +620,8 @@ Section CompatibilityLemmas.
     assert (es : S.fixt (repEmul τ₁) (repEmul τ₂) (S.abs (repEmul (ptarr τ₁ τ₂)) tsb) --> tsb [beta1 (S.abs (repEmul τ₁) (S.app (S.fixt (repEmul τ₁) (repEmul τ₂) (S.abs (repEmul τ₁ ⇒ repEmul τ₂) tsb[wkm↑])) (S.var 0)))]) by (refine (eval_ctx₀ S.phole _ _); crush).
     assert (es1 : S.evaln (S.fixt (repEmul τ₁) (repEmul τ₂) (S.abs (repEmul (ptarr τ₁ τ₂)) tsb)) (tsb [beta1 (S.abs (repEmul τ₁) (S.app (S.fixt (repEmul τ₁) (repEmul τ₂) (S.abs (repEmul τ₁ ⇒ repEmul τ₂) tsb[wkm↑])) (S.var 0)))])  1) by 
         (eauto using S.evaln; omega).
-    assert (es2 : forall Cu, U.ECtx Cu → U.evaln (U.pctx_app (U.ufix₁ (U.abs tub)) Cu) (U.pctx_app (tub[beta1 (U.abs (U.app (U.ufix₁ (U.abs tub[wkm↑])) (U.var 0)))]) Cu) 2) by
-        (intros Cu eCu; eauto using U.evaln, U.ufix₁_evaln').
+    assert (es2 : U.ctxevaln (U.ufix₁ (U.abs tub)) (tub[beta1 (U.abs (U.app (U.ufix₁ (U.abs tub[wkm↑])) (U.var 0)))]) 2) by
+        (eauto using U.ufix₁_evaln' with eval).
     destruct w; try apply termrel_zero.
     refine (termrel_antired w es1 es2 _ _ _); unfold lev in *; simpl; try omega.
     clear es es1 es2.
@@ -668,8 +670,8 @@ Section CompatibilityLemmas.
     (* next, reduce (U.app U.ufix tu) by one step in the conclusion *)
     assert (es1 : S.evaln (S.fixt (repEmul τ₁) (repEmul τ₂) vs) (S.fixt (repEmul τ₁) (repEmul τ₂) vs) 0) by
         (eauto using S.evaln).
-    assert (es2 : forall Cu, U.ECtx Cu → U.evaln (U.pctx_app (U.app U.ufix vu) Cu) (U.pctx_app (U.ufix₁ vu) Cu) 1) 
-      by (intros Cu eCu; eauto using U.evaln, U.ufix_eval₁').
+    assert (es2 : U.ctxevaln (U.app U.ufix vu) (U.ufix₁ vu) 1) 
+      by (unfold U.ctxevaln; eauto using U.ufix_eval₁' with eval).
     refine (termrel_antired w' es1 es2 _ _ _); unfold lev in *; simpl; try omega. 
 
     (* then defer to valrel_fix *) 
