Compiler/ProtectConfine.v
@@ -4,9 +4,13 @@ Require Stlc.SpecTyping.
 Require Stlc.LemmasTyping.
 Require Import Utlc.SpecSyntax.
 Require Import Utlc.SpecEvaluation.
+Require Import Utlc.LemmasEvaluation.
 Require Import Utlc.LemmasScoping.
+Require Import Utlc.Inst.
+Require Import Utlc.DecideEval.
 Require Import LogRel.PseudoType.
 Require Import LogRel.LR.
+Require Import LogRel.LemmasLR.
 Require Import Erase.
 
 Module S.
@@ -56,13 +60,16 @@ Local Ltac crush :=
           S.crushTyping
          ).
   
-Lemma protect_confine_closed {τ} :
+Lemma protect_confine_closed τ :
   ⟨ 0 ⊢ protect τ ⟩ ∧ 
   ⟨ 0 ⊢ confine τ ⟩.
 Proof.
-  induction τ; simpl; crush.
-  (* weakening for well-scopedness *)
-Admitted.
+  induction τ; simpl; crush;
+  try match goal with
+      [ H : ⟨ 0 ⊢ ?t ⟩ |- ⟨ ?d ⊢ ?t ⟩ ] => (rewrite <- (wsClosed_invariant H (wkms d));
+                                            exact (weakenings d H))
+  end.
+Qed.
   
 Lemma protect_confine_terminate {τ vu} :
   OfTypeUtlc (embed τ) vu →
@@ -73,17 +80,42 @@ Proof.
   revert vu.
   induction τ; crush.
   - (* ptarr τ₁ τ₂ *)
-    exists (abs (app (protect τ2) (app vu (app (confine τ1) (var 0))))).
+    exists (abs (app (protect τ2) (app vu[wkm] (app (confine τ1) (var 0))))).
     crush. 
     enough (U.pctx_app
               (U.app
                  (abs (abs (app (protect τ2) (app (var 1) (app (confine τ1) (var 0))))))
                  vu) Cu -->
-              U.pctx_app (abs (app (protect τ2) (app vu (app (confine τ1) (var 0))))) Cu) by eauto with eval.
+              U.pctx_app (abs (app (protect τ2) (app vu[wkm] (app (confine τ1) (var 0))))) Cu) by eauto with eval.
     refine (U.eval_ctx₀ _ _ _); crush.
-    replace (abs (app (protect τ2) (app vu (app (confine τ1) (var 0))))) with ((abs (app (protect τ2) (app (var 1) (app (confine τ1) (var 0))))) [beta1 vu]).
+    replace (abs (app (protect τ2) (app vu[wkm] (app (confine τ1) (var 0))))) with 
+      ((abs (app (protect τ2) (app (var 1) (app (confine τ1) (var 0))))) [beta1 vu]).
     + refine (U.eval_beta _); crush.
-    + simpl. repeat f_equal.
+    + pose (protect_confine_closed τ2).
+      pose (protect_confine_closed τ1).
+      crush; eauto using wsClosed_invariant.
+      (* vu[wkm] = vu[wkm]:  applying the weakening substitution is the same as the renaming: lemma missing? *)
+      admit.
+  - (* ptunit *)
+    exists unit; crush.
+    eapply evaln_to_evalStar.
+    subst; apply (evalMax 10 (app (abs (var 0)) unit) nil (idm UTm)); crush.
+  - (* ptbool *)
+    exists true; crush.
+    eapply evaln_to_evalStar.
+    subst; apply (evalMax 10 (app (abs (var 0)) true) nil (idm UTm)); crush.
+  - (* ptbool *)
+    exists false; crush.
+    eapply evaln_to_evalStar.
+    subst; apply (evalMax 10 (app (abs (var 0)) false) nil (idm UTm)); crush.
+  - destruct H as [t₁ [t₂ [eq [ot1 ot2]]]]; subst.
+    destruct (IHτ1 t₁ ot1) as [v1 [vv1 e1]].
+    destruct (IHτ2 t₂ ot2) as [v2 [vv2 e2]].
+    exists (pair v1 v2); crush.
+    
+
+    
+        
       (* Problem: no assumption currently that OfType values are closed *) 
       (* Problem: closedness implies that substitution has no effect: lemma missing? *) 
 Admitted.
